

8 Lesson 8

8.1 The Product Rule

Example 1: Suppose $f(x) = 3x^3(5x^2 + 7x)$. Find $f'(x)$.

$$f(x) = 15x^5 + 21x^4$$

$$f'(x) = 75x^4 + 84x^3$$

What happens if we take the derivative of each factor and multiply them together?

$$f'(x) \stackrel{?}{=} 9x^2(10x + 7) = 90x^3 + 63x^2 \quad \leftarrow \text{No!}$$

$$\frac{d}{dx}[f(x)g(x)] \neq \left[\frac{d}{dx}f(x) \right] \left[\frac{d}{dx}g(x) \right]$$

Using the limit definition of a derivative (and some cleverness), we can show that

$$\frac{d}{dx}[f(x)g(x)] = \left[\frac{d}{dx}f(x) \right] g(x) + \left[\frac{d}{dx}g(x) \right] f(x). \quad (*)$$

Example 1 (revisited): Suppose $y = 3x^3(5x^2 + 7x)$. Find y' using the product rule.

$$f(x) = 3x^3$$

$$g(x) = 5x^2 + 7x$$

$$f'(x) = 9x^2$$

$$g'(x) = 10x + 7$$

$$y' = f'(x)g(x) + g'(x)f(x)$$

$$= 9x^2(5x^2 + 7x) + (10x + 7)3x^3$$

$$= 45x^4 + 63x^3 + 30x^4 + 21x^3$$

$$= 75x^4 + 84x^3$$

Example 2: Find the derivative of $y = 3e^x \cos(x)$ at $x = \pi$.

$$f(x) = 3e^x$$

$$g(x) = \cos(x)$$

$$f'(x) = 3e^x$$

$$g'(x) = -\sin(x)$$

$$y' = f'(x)g(x) + g'(x)f(x)$$

$$= 3e^x \cos(x) - \sin(x) \cdot 3e^x$$

$$= 3e^x (\cos(x) - \sin(x))$$

$$y'(\pi) = 3e^\pi (\underbrace{\cos(\pi)}_{-1} - \underbrace{\sin(\pi)}_0) = -3e^\pi$$

8.2 Practice Problems

1. Find the x -values at which $y = 6x^8 e^x$ has a horizontal tangent line.

$$f(x) = 6x^8$$

$$g(x) = e^x$$

where tangent line
has slope 0, i.e.
where deriv. is 0

$$y' = 48x^7 e^x + e^x 6x^8$$

$$= 6x^7 e^x (8 + x)$$

$$\text{Solve } 0 = 6x^7 e^x (8 + x)$$

$$\Rightarrow 6x^7 e^x = 0$$

$$8 + x = 0$$

$$\Rightarrow \begin{matrix} x = 0 \\ x = -8 \end{matrix}$$

2. Find the equation of the tangent line to the curve of $y = 7x \sin(x)$ at $x = \pi$.

$$y' = 7\sin(x) + \cos(x) 7x$$

$$y'(\pi) = \underbrace{7\sin(\pi)}_0 + \underbrace{\cos(\pi)}_{-1} \cdot 7\pi = -7\pi \leftarrow \text{slope}$$

$$y(\pi) = 7\pi \sin(\pi) = 0$$

\hookrightarrow pt. is $(\pi, 0)$

$$y - 0 = -7\pi(x - \pi)$$

$$\Rightarrow y = -7\pi x + 7\pi^2$$

proof of (*):

def. of derivative

$$\frac{d}{dx} (f(x)g(x)) = \lim_{h \rightarrow 0} \frac{f(x+h)g(x+h) - f(x)g(x)}{h}$$

add "0"

$$= \lim_{h \rightarrow 0} \frac{f(x+h)g(x+h) - f(x+h)g(x) + f(x+h)g(x) - f(x)g(x)}{h}$$

$$= \lim_{h \rightarrow 0} \frac{f(x+h)g(x+h) - f(x+h)g(x)}{h} + \lim_{h \rightarrow 0} \frac{f(x+h)g(x) - f(x)g(x)}{h}$$

$$= \lim_{h \rightarrow 0} f(x+h) \left[\frac{g(x+h) - g(x)}{h} \right] + \lim_{h \rightarrow 0} g(x) \left[\frac{f(x+h) - f(x)}{h} \right]$$

$$= \lim_{h \rightarrow 0} f(x+h) \cdot \lim_{h \rightarrow 0} \left[\frac{g(x+h) - g(x)}{h} \right] + g(x) \cdot \lim_{h \rightarrow 0} \left[\frac{f(x+h) - f(x)}{h} \right]$$

$$= f(x)g'(x) + g(x)f'(x)$$